src/Compiler.v
@@ -2,13 +2,18 @@ Require Import Common.
 Require Import Language.
 Require Import Assembly.
 
-Require Import List.
-Import ListNotations.
+Require Import Vector.
+Import Vector.VectorNotations.
+Require Import Program.Equality.
 Require Import PeanoNat.
+Require Import Lia.
 Import Nat.
+Require Import Coq.Vectors.VectorEq.
+
 Module Compiler.
 
-Fixpoint matched' (p : Language.program) (c : nat) : bool :=
+Definition lenvec {A n} (v : Vector.t A n) : nat := n.
+Fixpoint matched' {n} (p : Language.program n) (c : nat) : bool :=
   match c with
   | 0 => false
   | _ => match p with
@@ -19,96 +24,181 @@ Fixpoint matched' (p : Language.program) (c : nat) : bool :=
     end
   end.
 
-Inductive matched (p : Language.program) : Prop :=
+Inductive matched {n} (p : Language.program n) : Prop :=
   | match_r : matched' p 1 = true -> matched p.
+Fixpoint comp_len {n} (p : Language.program n) : nat :=
+  match p with
+  | Vector.nil _ => 0
+  | Language.PtrInc :: xs => 1 + comp_len xs
+  | Language.PtrDec :: xs => 1 + comp_len xs
+  | Language.Inc :: xs => 6 + comp_len xs
+  | Language.Dec :: xs => 6 + comp_len xs
+  | Language.Jump :: xs => 2 + comp_len xs
+  | Language.Ret :: xs => 2 + comp_len xs
+  | Language.Halt :: xs => 1 + comp_len xs
+  end.
 
-(* won't compute new addresses *)
-Fixpoint compile'' (p : Language.program): (Assembly.program) :=
+Fixpoint compile''_ {n n'} (p : Language.program n) :
+                          (Assembly.program' (comp_len p) n') :=
   match p with
   | [] => []
-  | Language.PtrInc :: t => (Assembly.Add 1) :: compile'' t
-  | Language.PtrDec :: t => (Assembly.Sub 1) :: compile'' t
-  | Language.Inc :: t =>  Assembly.Swap   ::
+  | Language.PtrInc :: h => (Assembly.Add 1) :: compile''_ h
+  | Language.PtrDec :: h => (Assembly.Sub 1) :: compile''_ h
+  | Language.Inc :: h =>  Assembly.Swap   ::
                           Assembly.Load   ::
                           Assembly.Add 1  ::
                           Assembly.Store  ::
                           Assembly.Zero   ::
-                          Assembly.Swap   :: compile'' t
-  | Language.Dec :: t =>  Assembly.Swap   ::
+                          Assembly.Swap   :: compile''_ h
+  | Language.Dec :: h =>  Assembly.Swap   ::
                           Assembly.Load   ::
                           Assembly.Sub 1  ::
                           Assembly.Store  ::
                           Assembly.Zero   ::
-                          Assembly.Swap   :: compile'' t
+                          Assembly.Swap   :: compile''_ h
 
-  | Language.Jump :: t => Assembly.Skip   ::
-                          Assembly.Jump 0 :: compile'' t
-  | Language.Ret :: t =>  Assembly.Skip   ::
-                          Assembly.Jump 1 :: compile'' t
-  | Language.Halt :: t => Assembly.Halt   :: compile'' t
+  | Language.Jump :: h => Assembly.Skip   ::
+                          Assembly.UJUMP :: compile''_ h
+  | Language.Ret :: h =>  Assembly.Skip   ::
+                          Assembly.URET :: compile''_ h
+  | Language.Halt :: h => Assembly.Halt   :: compile''_ h
   end.
 
-Fixpoint new_pc' (p : Language.program) (pc c c' : nat) : nat :=
+Definition compile_first {n : nat} (i : Language.instr) : Assembly.instr (n:=n) :=
+  match i with
+  | Language.PtrInc => Assembly.Add 1
+  | Language.PtrDec => Assembly.Sub 1
+  | Language.Inc => Assembly.Swap
+  | Language.Dec => Assembly.Swap
+  | Language.Jump => Assembly.Skip
+  | Language.Ret => Assembly.Skip
+  | Language.Halt => Assembly.Halt
+  end.
+Definition compile'' {n} (p : Language.program n) : (Assembly.program (comp_len p)) := 
+  @compile''_ n (comp_len p) p.
+
+Fixpoint compile_index {n} (p : Language.program n) (x : Fin.t n) : Fin.t (comp_len p).
+Proof.
+  destruct x eqn:H1; rewrite (eta p).
+  - destruct hd; apply Fin.F1.
+  - destruct hd.
+    + do 1 apply Fin.FS. apply compile_index. exact t0.
+    + do 1 apply Fin.FS. apply compile_index. exact t0.
+    + do 6 apply Fin.FS. apply compile_index. exact t0.
+    + do 6 apply Fin.FS. apply compile_index. exact t0.
+    + do 2 apply Fin.FS. apply compile_index. exact t0.
+    + do 2 apply Fin.FS. apply compile_index. exact t0.
+    + do 1 apply Fin.FS. apply compile_index. exact t0.
+Defined.
+
+Fixpoint nb_jump' {n n'} (p : Assembly.program' n n') : nat :=
   match p with
   | [] => 0
-  | Language.PtrInc :: t => if c =? pc then c' else new_pc' t pc (c+1) (c'+1)
-  | Language.PtrDec :: t => if c =? pc then c' else new_pc' t pc (c+1) (c'+1)
-  | Language.Inc :: t =>    if c =? pc then c' else new_pc' t pc (c+1) (c'+6)
-  | Language.Dec :: t =>    if c =? pc then c' else new_pc' t pc (c+1) (c'+6)
-  | Language.Jump :: t =>   if c =? pc then c' else new_pc' t pc (c+1) (c'+2)
-  | Language.Ret :: t =>    if c =? pc then c' else new_pc' t pc (c+1) (c'+2)
-  | Language.Halt :: t =>   if c =? pc then c' else new_pc' t pc (c+1) (c'+1)
+  | Assembly.UJUMP :: t => 1 + nb_jump' t
+  | _ :: t => nb_jump' t
   end.
 
-Definition new_pc (p : Language.program) (pc : nat) : nat := new_pc' p pc 0 0.
+Definition nb_jump {n} (p : Assembly.program n) : nat := @nb_jump' n n p.
 
-Definition safe_head (p : list nat) : nat :=
+Fixpoint nb_ret' {n n'} (p : Assembly.program' n n') : nat :=
   match p with
   | [] => 0
-  | h :: l => h
-  end. (* no risk of unmatched jump / ret, thanks to `matched` *)
+  | Assembly.URET :: t => 1 + nb_ret' t
+  | _ :: t => nb_ret' t
+  end.
 
-Fixpoint link_ret' (p : Assembly.program) (pos : nat) (c : list nat) : Assembly.program :=
+Definition nb_ret {n} (p : Assembly.program n) : nat := @nb_ret' n n p.
+
+Definition vector_zip {n : nat} (A : Type) (v1 v2 : Vector.t A n) : Vector.t (A * A) n :=
+  Vector.map2 (fun x y => (x,y)) v1 v2.
+
+Fixpoint j_indexes' {n n'} (p : Assembly.program' n n') : (Vector.t (Fin.t n) (nb_jump' p)) :=
   match p with
   | [] => []
-  | Assembly.Jump 0 :: t => Assembly.Jump 0 :: link_ret' t (pos+1) (pos::c)
-  | Assembly.Jump 1 :: t => Assembly.Jump (safe_head c + 1) :: link_ret' t (pos+1) (tail c)
-  | i :: t => i :: link_ret' t (pos+1) c 
+  | Assembly.UJUMP :: t => Fin.F1 :: map Fin.FS (j_indexes' t)
+  | _ :: t => map Fin.FS (j_indexes' t)
   end.
 
-Definition link_ret (p : Assembly.program) : Assembly.program := link_ret' p 0 [].
+Definition j_indexes {n} (p : Assembly.program n) : Vector.t (Fin.t n) (nb_jump p) :=
+  j_indexes' p.
 
-Fixpoint get_index (l: Assembly.program) (start_idx: nat) (c : nat) : option nat :=
-  match l with
-  | [] => None
-  | Assembly.Jump 0 :: t => get_index t (start_idx + 1) (c + 1)
-  | Assembly.Jump _ :: t => if c =? 0 then Some start_idx else get_index t (start_idx + 1) (c - 1)
-  | _ :: t => get_index t (start_idx + 1) c
-  end.
-
-Fixpoint link_jump' (l: Assembly.program) (idx : nat) : Assembly.program :=
-  match l with
+Fixpoint r_indexes' {n n'} (p : Assembly.program' n n') : (Vector.t (Fin.t n) (nb_ret' p)) :=
+  match p with
   | [] => []
-  | h :: t => match h with
-              | Assembly.Jump 0 => match get_index t (idx + 1) 0 with
-                                   | Some i => Assembly.Jump (i + 1) :: link_jump' t (idx + 1)
-                                   | None   => h :: link_jump' t (idx + 1)
-                                   end
-              | _ => h :: link_jump' t (idx + 1)
-              end
+  | Assembly.URET :: t => Fin.F1 :: map Fin.FS (r_indexes' t)
+  | _ :: t => map Fin.FS (r_indexes' t)
   end.
 
-Definition link_jump (l : Assembly.program) : Assembly.program := link_jump' l 0.
+Definition r_indexes {n} (p : Assembly.program n) : Vector.t (Fin.t n) (nb_ret p) :=
+  r_indexes' p.
 
-Definition link (l : Assembly.program) : Assembly.program := link_jump (link_ret l).
+Fixpoint link_jump' {n ln ln'} (p : Assembly.program n) 
+                          (jumps : Vector.t (Fin.t n) ln) (rets : Vector.t (Fin.t n) ln') :
+                          Assembly.program n :=
+  match jumps with
+  | [] => p
+  | a :: jumps' => match rets with
+                  | [] => p
+                  | r :: rets' => link_jump' (replace p a (Assembly.Jump r)) jumps' rets'
+                  end
+  end.
 
-Definition compile' (p : Language.state) : Assembly.state :=
-  Assembly.mkState (link (compile'' p.(Language.prog))) p.(Language.mem)
-                   (new_pc p.(Language.prog) p.(Language.pc)) p.(Language.ptr) 0.
 
-Compute (link (compile'' [Language.PtrInc; Language.Jump; Language.Halt; Language.Halt; Language.Ret])).
+Definition link_jump {n} (p : Assembly.program n) : (Assembly.program n) :=
+  link_jump' p (j_indexes p) (r_indexes p).
 
-Inductive compile (p : Language.state) (q : Assembly.state) : Prop :=
-  | comp_r : matched p.(Language.prog) -> q = compile' p -> compile p q.
+Definition link_ret {n} (p : Assembly.program n) : (Assembly.program n).
+Admitted. (* todo *)
 
+Definition link {n} (l : Assembly.program n) : (Assembly.program n) := link_ret (link_jump l) .
+
+Definition make_vector (A : Type) (x : A) (n : nat) : Vector.t A n.
+Proof.
+  induction n.
+  - apply Vector.nil.
+  - apply Vector.cons.
+    + exact x.
+    + exact IHn.
+Defined.
+
+Definition make_f1 (x : nat) (H : x <> 0) : Fin.t x.
+Proof.
+  destruct x eqn:H1.
+  - auto with *.
+  - exact Fin.F1.
+Defined.
+
+Lemma lm1 {n} : forall p, n <> 0 -> comp_len (@Language.prog n p) <> 0.
+Proof.
+  intros.
+  destruct p.
+  cbn.
+  destruct prog.
+  inversion pc.
+  unfold not. intros.
+  destruct h; inversion H0.
+Qed.
+Lemma lm2 : 512 <> 0.
+Proof. lia. Qed.
+
+Definition compile' {n}
+  (p : Language.state (n := n)) (HA: n <> 0) : 
+  (Assembly.state (n := comp_len p.(Language.prog)) (m := 512)) :=
+  let newlen := comp_len p.(Language.prog) in
+  let newpc := compile_index p.(Language.prog) p.(Language.pc) in
+  let f1_index := make_f1 (comp_len p.(Language.prog)) (lm1 p HA) in
+  let f1_mem := make_f1 512 lm2 in
+  @Assembly.mkState newlen 512 (compile'' p.(Language.prog)) p.(Language.mem) newpc f1_mem p.(Language.ptr).
+
+Definition compile_link {n} (p : Language.state (n := n)) (HA : n <> 0) : 
+  (Assembly.state (n := comp_len p.(Language.prog)) (m := 512)) :=
+  let cpl := compile' p HA in
+  Assembly.mkState (comp_len (Language.prog p)) 512 (link cpl.(Assembly.prog)) cpl.(Assembly.mem) cpl.(Assembly.pc) cpl.(Assembly.ac) cpl.(Assembly.b).
+
+Compute (link [Assembly.UJUMP; Assembly.URET]).
+
+Inductive compile {n}
+  (p : Language.state (n := n))
+  (q : Assembly.state (n := comp_len p.(Language.prog)) (m := 512)) : Prop :=
+  | comp_r : forall H, matched (p.(Language.prog)) -> q = compile_link p H -> compile p q.
 End Compiler.
