src/Language.v
@@ -1,8 +1,9 @@
-Require Import List.
-Import ListNotations.
-Require Import Common.
+Require Import Vector.
+Import Vector.VectorNotations.
+Require Import Program.Equality.
 Require Import PeanoNat.
-Import Nat.
+Require Import Common.
+Require Import Lia.
 Module Language.
 Inductive instr : Type :=
   | PtrInc : instr
@@ -12,81 +13,97 @@ Inductive instr : Type :=
   | Jump : instr
   | Ret : instr
   | Halt : instr.
-Definition program := list instr.
+Definition program (n : nat) := t instr n.
 
-Record state : Type := mkState
+Record state {n : nat} : Type := mkState
 { 
-  prog : program;
-  mem : list nat;
-  pc : nat;
-  ptr : nat;
+  prog : program n;
+  mem : t nat 512;
+  pc : Fin.t n;
+  ptr : Fin.t 512;
 }.
 
-Fixpoint read_instr' (prog : program) (pc : nat) : instr :=
-  match prog, pc with
-  | [], _ => Halt
-  | i :: _, 0 => i
-  | _ :: t, S pc' => read_instr' t pc'
+Definition read_instr' {n} (prog : program n) (pc : Fin.t n) : instr := prog[@pc].
+
+Inductive read_instr {n} (p : state) (i : instr) : Prop  :=
+  | ri : read_instr' p.(prog n) p.(pc n) = i -> read_instr p i.
+
+Definition read_mem' (mem : t nat 512) (ptr : Fin.t 512) : nat := mem[@ptr].
+
+Inductive read_mem {n} (p : state) (e : nat) : Prop  :=
+  | mi : read_mem' p.(mem n) p.(ptr n) = e -> read_mem p e.
+
+Fixpoint to_nat {n} (x : Fin.t n) : nat.
+Proof.
+  destruct x eqn:H.
+  - exact 0.
+  - apply plus.
+    + exact 1.
+    + apply to_nat with (n := n).
+      exact t.
+Defined.
+
+Inductive mem_diff {m} (m1 : t nat m) (m2 : t nat m) (x : Fin.t m) : Prop :=
+  | md : (forall i, i <> x -> m2[@i] = m1[@i]) -> mem_diff m1 m2 x. 
+
+Fixpoint matching_ret' {n} (l : t instr n) (idx : nat) (c c' : nat) : option nat :=
+  match l with
+  | [] => None
+  | i :: h => if c' <=? idx then matching_ret' h idx c (c'+1) else
+    match i with
+    | Jump => matching_ret' h idx (c+1) (c'+1)
+    | Ret => if c =? 0 then Some c' else matching_ret' h idx (c-1) (c'+1)
+    | _ => matching_ret' h idx c (c'+1)
+  end
+end.
+
+Fixpoint matching_jump' {n} (l : t instr n) (idx : nat) (c : nat) (c' : option nat) : option nat :=
+  match l with
+  | [] => None
+  | Jump :: h => if c =? idx then None else matching_jump' h idx (c+1) (Some c)
+  | Ret :: h => if c =? idx then c' else None
+  | _ :: h => if c =? idx then None else matching_jump' h idx (c+1) c'
   end.
 
-Inductive read_instr (p : state) (i : instr) : Prop  :=
-  | ri : read_instr' p.(prog) p.(pc) = i -> read_instr p i.
-
-Fixpoint read_mem' (m : list nat) (index : nat) : nat :=
-  match m, index with
-  | [], _ => 0
-  | i :: _, 0 => i
-  | _ :: t, S index' => read_mem' t index'
-  end.
-
-Inductive read_mem (p : state) (n : nat) : Prop  :=
-  | mi : read_mem' p.(mem) p.(ptr) = n -> read_mem p n.
-
-Inductive mem_diff_p (m : list nat) (m' : list nat) (ptr : nat) : Prop :=
-  | c_diff_p : Common.take ptr m = Common.take ptr m' ->
-               Common.drop (ptr+1) m = Common.drop (ptr+1) m' ->
-               Common.drop (ptr) (Common.take (ptr+1) m') = (map (fun x => x + 1))
-               (Common.drop (ptr) (Common.take (ptr+1) m)) 
-               -> mem_diff_p m m' ptr.
-
-Inductive mem_diff_m (m : list nat) (m' : list nat) (ptr : nat) : Prop :=
-  | c_diff_m : Common.take ptr m = Common.take ptr m' ->
-               Common.drop (ptr+1) m = Common.drop (ptr+1) m' ->
-               Common.drop (ptr) (Common.take (ptr+1) m') = (map (fun x => x - 1))
-               (Common.drop (ptr) (Common.take (ptr+1) m)) 
-               -> mem_diff_m m m' ptr.
+Inductive matching_jump {n} (p : program n) (x : Fin.t n) (x' : Fin.t n) : Prop :=
+  | mj : matching_jump' p (to_nat x) 0 None = Some (to_nat x') -> matching_jump p x x'.
+Inductive matching_ret {n} (p : program n) (x : Fin.t n) (x' : Fin.t n): Prop :=
+  | mr : matching_ret' p (to_nat x) 0 0 = Some (to_nat x') -> matching_ret p x x'.
 
 (*Some cases will not be accepted for compilation anyway, like unmatched jumps.*)
 (* Small-step operational semantics for our source language.*)
-Inductive semantics (p : state) (p' : state) : Prop :=
-  | ptr_inc : read_instr p PtrInc -> p.(ptr) + 1 = p'.(ptr) ->
-                   p.(pc) + 1 = p'.(pc) -> p.(prog) = p'.(prog) ->
-                   p.(mem) = p'.(mem) -> semantics p p' 
-  | ptr_dec : read_instr p PtrDec -> p.(ptr) - 1 = p'.(ptr) ->
-                   p.(pc) + 1 = p'.(pc) -> p.(prog) = p'.(prog) ->
+
+Inductive semantics {n} (p : state) (p' : state) : Prop :=
+  | ptr_inc : read_instr p PtrInc ->  to_nat p.(ptr) + 1 = to_nat p'.(ptr) ->
+                   to_nat p.(pc n) + 1 = to_nat p'.(pc)-> p.(prog) = p'.(prog) ->
+                   p.(mem) = p'.(mem) -> semantics p p'
+  | ptr_dec : read_instr p PtrDec -> to_nat p.(ptr) - 1 = to_nat p'.(ptr) ->
+                    to_nat p.(pc) +1 = to_nat p'.(pc)-> p.(prog) = p'.(prog) ->
                    p.(mem) = p'.(mem) -> semantics p p'
   | inc : read_instr p Inc -> p.(ptr) = p'.(ptr) ->
-               length p.(mem) > p.(ptr) ->
-               p.(pc) + 1 = p'.(pc) -> p.(prog) = p'.(prog) ->
-               mem_diff_p p.(mem) p'.(mem) p.(ptr) -> semantics p p' 
+               to_nat p.(pc) +1 = to_nat p'.(pc)-> p.(prog) = p'.(prog) ->
+               mem_diff p.(mem) p'.(mem) p.(ptr) ->
+               p.(mem)[@p.(ptr)] + 1 = p'.(mem)[@p.(ptr)] ->
+               semantics p p'
   | dec : read_instr p Dec -> p.(ptr) = p'.(ptr) ->
-               length p.(mem) > p.(ptr) ->
-               p.(pc) + 1 = p'.(pc) -> p.(prog) = p'.(prog) ->
-               mem_diff_m p.(mem) p'.(mem) p.(ptr) -> semantics p p' 
+               to_nat p.(pc) +1 = to_nat p'.(pc)-> p.(prog) = p'.(prog) ->
+               mem_diff p.(mem) p'.(mem) p.(ptr) ->
+               p.(mem)[@p.(ptr)] - 1 = p'.(mem)[@p.(ptr)] ->
+               semantics p p'
   | jump_z : read_instr p Jump -> p.(ptr) = p'.(ptr) ->
                   p.(prog) = p'.(prog) -> p.(mem) = p'.(mem) ->
-                  length p.(mem) > p.(ptr) -> read_mem p 0 ->
+                  read_mem p 0 -> matching_ret p.(prog) p.(pc) p'.(pc) ->
                   semantics p p'
   | jump_nz : read_instr p Jump -> p.(ptr) = p'.(ptr) ->
                    p.(prog) = p'.(prog) -> p.(mem) = p'.(mem) ->
-                   length p.(mem) > p.(ptr) -> ~ (read_mem p 0) ->
-                   p.(pc) + 1 = p'.(pc) -> semantics p p'
+                   ~ (read_mem p 0) ->
+                   to_nat p.(pc) + 1 = to_nat p'.(pc)-> semantics p p'
   | ret_z :  read_instr p Ret -> p.(ptr) = p'.(ptr) ->
                   p.(prog) = p'.(prog) -> p.(mem) = p'.(mem) ->
-                  length p.(mem) > p.(ptr) -> read_mem p 0 ->
+                  matching_jump p.(prog) p.(pc) p'.(pc) -> read_mem p 0 ->
                   semantics p p'
   | ret_nz : read_instr p Ret -> p.(ptr) = p'.(ptr) ->
                   p.(prog) = p'.(prog) -> p.(mem) = p'.(mem) ->
-                  length p.(mem) > p.(ptr) -> ~ (read_mem p 0) ->
-                  p.(pc) + 1 = p'.(pc) -> semantics p p'.
+                  ~ (read_mem p 0) ->
+                  to_nat p.(pc) +  1 = to_nat p'.(pc) -> semantics p p'.
 End Language.
