src/Verification.v
@@ -3,724 +3,101 @@ Require Import Language.
 Require Import Assembly.
 Require Import Simulation.
 Require Import Compiler.
-Require Import List.
 Require Import Lia.
-Import ListNotations.
+Require Import Vector.
+Import Vector.VectorNotations.
+Require Import Program.Equality.
 Require Import PeanoNat.
 Import Nat.
-
-Require Import Coq.Program.Equality.
-
-From Hammer Require Import Hammer.
-From Hammer Require Import Tactics.
-From Hammer Require Import Reflect.
-
 Module Verification.
-Definition eval := Language.semantics.
-Definition eval' := Assembly.semantics.
 
-Theorem constant_code : forall p p', eval p p' -> p.(Language.prog) = p'.(Language.prog).
-Proof.
-  intros.
-  inversion H; assumption.
-Qed.
-Theorem constant_asm' : forall q q', eval' q q' -> q.(Assembly.prog) = q'.(Assembly.prog).
-Proof.
-  intros.
-  inversion H; assumption.
-Qed.
-Theorem constant_asm : forall p p' q q', Compiler.compile p q -> Compiler.compile p' q' ->
-                       eval p p' -> q.(Assembly.prog) = q'.(Assembly.prog).
-Proof.
-  intros.
-  inversion H.
-  inversion H0.
-  unfold Compiler.compile' in H3, H5.
-  rewrite H3.
-  rewrite H5.
-  simpl.
-  assert (Language.prog p = Language.prog p').
-  apply constant_code.
-  assumption.
-  rewrite H6.
-  reflexivity.
-Qed.
+Definition eval {n} := @Language.semantics n.
+Definition eval' {n} := @Assembly.semantics n 512.
 
-Theorem match_preserve : 
-  forall p p', Language.semantics p p' ->
-               Compiler.matched (Language.prog p) ->
-               Compiler.matched (Language.prog p').
+Lemma comp_len_eq : forall n p p', eval p p' -> @Compiler.comp_len n (@Language.prog n p) = @Compiler.comp_len n (@Language.prog n p').
 Proof.
   intros.
   assert (p.(Language.prog) = p'.(Language.prog)).
-  - apply constant_code.
+  + inversion H; assumption.
+  + inversion H0.
+    reflexivity.
+Defined.
+
+Definition comp_len_f {n p p'} (H : eval p p') (q : @Assembly.state (@Compiler.comp_len n (@Language.prog n p')) 512) : @Assembly.state (@Compiler.comp_len n (@Language.prog n p)) 512.
+Proof.
+  assert (@Compiler.comp_len n (@Language.prog n p) = @Compiler.comp_len n (@Language.prog n p')).
+  - apply comp_len_eq.
     assumption.
-  - destruct p, p'.
-    simpl in H1.
-    simpl.
-    simpl in H0.
-    rewrite H1 in H0.
+  - rewrite H0.
+    exact q.
+Defined.
+Definition comp_len_f' {n p p'} (H : eval p p') (q : @Assembly.state (@Compiler.comp_len n (@Language.prog n p)) 512) : @Assembly.state (@Compiler.comp_len n (@Language.prog n p')) 512.
+Proof.
+  assert (@Compiler.comp_len n (@Language.prog n p) = @Compiler.comp_len n (@Language.prog n p')).
+  - apply comp_len_eq.
     assumption.
-Qed.
+  - rewrite <- H0.
+    exact q.
+Defined.
   
-Definition first_comp_instr (i : Language.instr) : Assembly.instr :=
-  match i with
-  | Language.PtrInc => Assembly.Add 1
-  | Language.PtrDec => Assembly.Sub 1
-  | Language.Inc => Assembly.Swap
-  | Language.Dec => Assembly.Swap
-  | Language.Jump => Assembly.Skip
-  | Language.Ret => Assembly.Skip
-  | Language.Halt => Assembly.Halt
-  end.
-
-(* unnecessary
-Theorem first_instr_comp' : 
-  forall p q i x, Compiler.compile p q ->
-  Language.read_instr' p.(Language.prog) x = i ->
-  Assembly.read_instr' q.(Assembly.prog) (Compiler.new_pc p.(Language.prog) x)
-  = (first_comp_instr i).
-Proof.
-Admitted.
-*)
-
-
-(* A minimal version is available in prototype/Example.v *)
-
-
-Theorem first_instr_comp : forall p q i, Compiler.compile p q ->
-                           Language.read_instr p i ->
-                           Assembly.read_instr q (first_comp_instr i).
+Lemma match_tr {n} : forall p p', Compiler.matched (n := n) (Language.prog p) -> eval p p' -> Compiler.matched (Language.prog p').
 Proof.
   intros.
-  inversion H.
-  inversion H0.
-  apply Assembly.ri.
-  rewrite H2.
-  rewrite <- H3.
-  generalize (Language.pc p) as x.
-  induction p; intro x; destruct x; unfold first_comp_instr.
-Admitted.
-
-Theorem comp_newstate :
-  forall p q, Compiler.compile p q ->
-              q.(Assembly.pc) = Compiler.new_pc (p.(Language.prog)) (p.(Language.pc)) /\
-              q.(Assembly.ac) = p.(Language.ptr) /\
-              q.(Assembly.mem) = p.(Language.mem) /\
-              q.(Assembly.b) = 0 /\
-              Assembly.read_instr q (first_comp_instr
-              (Language.read_instr' p.(Language.prog) p.(Language.pc))).
-Proof.
-  intros.
-  inversion H.
-  inversion H1.
-  unfold Compiler.compile'.
-  simpl.
-  split. reflexivity.
-  split. reflexivity.
-  split. reflexivity.
-  split. reflexivity.
-  apply first_instr_comp with (p := p).
-  destruct q.
-  inversion H2.
-  apply Compiler.comp_r.
-  assumption.
-  unfold Compiler.compile'.
-  reflexivity.
-  apply Language.ri.
-  reflexivity.
-Qed.
-Theorem comp_newstate' :
-  forall p q i, Compiler.compile p q -> Language.read_instr p i ->
-              q.(Assembly.pc) = Compiler.new_pc (p.(Language.prog)) (p.(Language.pc)) /\
-              q.(Assembly.ac) = p.(Language.ptr) /\
-              q.(Assembly.mem) = p.(Language.mem) /\
-              q.(Assembly.b) = 0 /\
-              Assembly.read_instr q (first_comp_instr i).
-Proof.
-  intros.
-  inversion H.
-  inversion H2.
-  unfold Compiler.compile'.
-  simpl.
-  split. reflexivity.
-  split. reflexivity.
-  split. reflexivity.
-  split. reflexivity.
-  inversion H0.
-  rewrite <- H4.
-  apply comp_newstate.
-  apply Compiler.comp_r.
-  assumption.
-  unfold Compiler.compile'.
-  reflexivity.
-Qed.
-Definition emitted_instr (i : Language.instr) : nat :=
-  match i with
-  | Language.PtrInc => 1
-  | Language.PtrDec => 1
-  | Language.Inc => 6
-  | Language.Dec => 6
-  | Language.Jump => 2
-  | Language.Ret => 2
-  | Language.Halt => 1
-  end.
-Compute (Compiler.new_pc [Language.PtrInc] 1 ).
-
-Theorem offset_newpc_lm :
-  forall p p',
-  eval p p' -> Compiler.new_pc (Language.prog p') (Language.pc p') =
-               Compiler.new_pc (Language.prog p) (Language.pc p) 
-               + length (Compiler.compile'' [Language.read_instr' (Language.prog p) (Language.pc p)]).
-Admitted.
-
-Theorem offset_newpc :
-  forall p p',
-  eval p p' -> Compiler.new_pc (Language.prog p') (Language.pc p') =
-               Compiler.new_pc (Language.prog p) (Language.pc p) 
-               + emitted_instr (Language.read_instr' p.(Language.prog) p.(Language.pc)).
-Proof.
-  intros.
-  assert (Compiler.new_pc (Language.prog p') (Language.pc p') =
-               Compiler.new_pc (Language.prog p) (Language.pc p) 
-               + length (Compiler.compile'' [Language.read_instr' (Language.prog p) (Language.pc p)])).
-  apply offset_newpc_lm. assumption.
-  destruct (length
-       (Compiler.compile''
-          [Language.read_instr' (Language.prog p)
-             (Language.pc p)])) eqn:HA.
-  ssimpl.
-  ssimpl.
-Qed.
-Lemma read_instr_functional : forall p i j,
-  Language.read_instr p i -> Language.read_instr p j -> i <> j -> False.
-Proof.
-  intros.
-  inversion H0.
-  inversion H.
-  assert ((Language.read_instr' (Language.prog p) (Language.pc p) = 
-             Language.read_instr' (Language.prog p) (Language.pc p))).
-  reflexivity.
-  rewrite <- H2 in H1.
-  rewrite <- H3 in H1.
-  contradiction.
-Qed.
-
-Theorem inc_instr_comp :
-  forall p q p', Compiler.compile p q -> eval p p' ->
-              Language.read_instr p Language.Inc ->
-              exists q1 q2 q3 q4 q5,
-              (Assembly.read_instr q1 Assembly.Load /\
-              Assembly.read_instr q2 (Assembly.Add 1) /\
-              Assembly.read_instr q3 Assembly.Store /\
-              Assembly.read_instr q4 Assembly.Zero /\
-              Assembly.read_instr q5 Assembly.Swap /\
-              eval' q q1 /\ eval' q1 q2 /\ eval' q2 q3 /\ eval' q3 q4 /\ eval' q4 q5).
-Proof.
-  intros.
-  assert (Assembly.read_instr q (first_comp_instr Language.Inc)).
-  apply first_instr_comp with (p := p). assumption. assumption.
-  simpl in H2.
-  inversion H.
-  assert (exists q0 q1 q2 q3 q4 q5,
-                              Assembly.read_instr q0 Assembly.Swap /\
-                              Assembly.read_instr q1 Assembly.Load /\
-                              Assembly.read_instr q2 (Assembly.Add 1) /\
-                              Assembly.read_instr q3 Assembly.Store /\
-                              Assembly.read_instr q4 Assembly.Zero /\
-                              Assembly.read_instr q5 Assembly.Swap).
-  admit; assumption.
-  destruct H5. destruct H5. destruct H5. destruct H5. destruct H5.
-  destruct H5.
-  exists x0. exists x1. exists x2. exists x3. exists x4.
-  destruct H5. destruct H6. destruct H7.
-  destruct H8. destruct H9.
-  split. assumption.
-  split. assumption.
-  split. assumption.
-  split. assumption.
-  split. assumption.
-  clear H5. clear x.
-Admitted.
-
-Theorem dec_instr_comp :
-  forall p q p', Compiler.compile p q -> eval p p' ->
-              Language.read_instr p Language.Dec ->
-              exists q1 q2 q3 q4 q5,
-              (Assembly.read_instr q1 Assembly.Load /\
-              Assembly.read_instr q2 (Assembly.Sub 1) /\
-              Assembly.read_instr q3 Assembly.Store /\
-              Assembly.read_instr q4 Assembly.Zero /\
-              Assembly.read_instr q5 Assembly.Swap /\
-              eval' q q1 /\ eval' q1 q2 /\ eval' q2 q3 /\ eval' q3 q4 /\ eval' q4 q5).
-Proof.
-  intros.
-  assert (Assembly.read_instr q (first_comp_instr Language.Dec)).
-  apply first_instr_comp with (p := p). assumption. assumption.
-  simpl in H2.
-  inversion H.
-  assert (exists q0 q1 q2 q3 q4 q5,
-                              Assembly.read_instr q0 Assembly.Swap /\
-                              Assembly.read_instr q1 Assembly.Load /\
-                              Assembly.read_instr q2 (Assembly.Sub 1) /\
-                              Assembly.read_instr q3 Assembly.Store /\
-                              Assembly.read_instr q4 Assembly.Zero /\
-                              Assembly.read_instr q5 Assembly.Swap).
-  admit; assumption.
-  destruct H5. destruct H5. destruct H5. destruct H5. destruct H5.
-  destruct H5.
-  exists x0. exists x1. exists x2. exists x3. exists x4.
-  destruct H5. destruct H6. destruct H7.
-  destruct H8. destruct H9.
-  split. assumption.
-  split. assumption.
-  split. assumption.
-  split. assumption.
-  split. assumption.
-  clear H5. clear x.
-Admitted.
-
-Theorem jump_instr_comp :
-  forall p q p', Compiler.compile p q -> eval p p' -> 
-                 Language.read_instr p Language.Jump ->
-                 (exists n q1, Assembly.read_instr q1 (Assembly.Jump n) /\ eval' q q1).
-Proof.
-Admitted.
-
-Theorem sequence_comp_ptrinc :
-  forall p p' q q', Compiler.compile p q -> eval p p' -> Compiler.compile p' q' ->
-              Language.read_instr p Language.PtrInc ->
-              Common.plus eval' q q'.
-Proof.
-  intros.
-  apply Common.t_base.
-  assert (Assembly.read_instr q (Assembly.Add 1)).
-  apply (comp_newstate' p q Language.PtrInc).
-  assumption.
-  assumption.
-  assert (Assembly.read_instr q' (first_comp_instr
-                                 (Language.read_instr' p'.(Language.prog) p'.(Language.pc)))).
-  apply (comp_newstate' p' q').
-  assumption.
-  apply Language.ri.
-  reflexivity.
-  unfold eval'.
-  apply (Assembly.add q) with (n := 1).
-  - assumption.
-  - assert (Assembly.pc q = (Compiler.new_pc p.(Language.prog) p.(Language.pc))).
-    inversion H.
-    inversion H6.
-    unfold Compiler.compile'.
-    simpl.
-    reflexivity.
-    assert (Assembly.pc q' = (Compiler.new_pc p'.(Language.prog) p'.(Language.pc))).
-    inversion H1.
-    unfold Compiler.compile' in H7.
-    inversion H1.
-    inversion H9.
-    unfold Compiler.compile'.
-    simpl.
-    reflexivity.
-    assert (Compiler.new_pc (Language.prog p') (Language.pc p') =
-            Compiler.new_pc (Language.prog p) (Language.pc p) + emitted_instr (Language.read_instr' p.(Language.prog) p.(Language.pc))).
-    inversion H2.
-    assert (emitted_instr (Language.read_instr' p.(Language.prog) p.(Language.pc)) = 1).
-    rewrite H7.
-    simpl.
-    reflexivity.
-    apply offset_newpc.
+  assert (Language.prog p = Language.prog p').
+  - inversion H0; assumption.
+  - rewrite <- H1.
     assumption.
-    rewrite H7 in H6.
-    inversion H2.
-    rewrite H8 in H6.
-    simpl in H6.
-    rewrite <- H5 in H6.
-    rewrite H6.
-    reflexivity.
-  - inversion H.
-    inversion H6.
-    unfold Compiler.compile'.
-    inversion H1.
-    inversion H9.
-    unfold Compiler.compile'.
-    simpl.
-    f_equal.
-    f_equal.
-    apply constant_code.
-    assumption.
-  - inversion H.
-    inversion H6.
-    unfold Compiler.compile'.
-    simpl.
-    assert (Language.mem p' = Language.mem p).
-    inversion H0.
-    rewrite H12. reflexivity.
-    exfalso.
-    apply (read_instr_functional _ _ _ H8 H2).
-    discriminate.
-    exfalso.
-    apply (read_instr_functional _ _ _ H8 H2).
-    discriminate.
-    exfalso.
-    apply (read_instr_functional _ _ _ H8 H2).
-    discriminate.
-    exfalso.
-    apply (read_instr_functional _ _ _ H8 H2).
-    discriminate.
-    exfalso.
-    apply (read_instr_functional _ _ _ H8 H2).
-    discriminate.
-    exfalso.
-    apply (read_instr_functional _ _ _ H8 H2).
-    discriminate.
-    exfalso.
-    apply (read_instr_functional _ _ _ H8 H2).
-    discriminate.
-    rewrite <- H8.
-    inversion H1.
-    inversion H10.
-    unfold Compiler.compile'.
-    simpl.
-    reflexivity.
-  - assert (Assembly.b q = 0).
-    inversion H.
-    inversion H6.
-    unfold Compiler.compile'.
-    simpl.
-    reflexivity.
-    assert (Assembly.b q' = 0).
-    inversion H1.
-    inversion H7.
-    unfold Compiler.compile'.
-    simpl.
-    reflexivity.
-    rewrite H5, H6.
-    reflexivity.
-  - inversion H.
-    inversion H6.
-    unfold Compiler.compile'.
-    simpl.
-    inversion H1.
-    inversion H9.
-    unfold Compiler.compile'.
-    simpl.
-    inversion H0.
-    rewrite H12.
-    reflexivity.
-    exfalso.
-    apply (read_instr_functional _ _ _ H11 H2).
-    discriminate.
-    exfalso.
-    apply (read_instr_functional _ _ _ H11 H2).
-    discriminate.
-    exfalso.
-    apply (read_instr_functional _ _ _ H11 H2).
-    discriminate.
-    exfalso.
-    apply (read_instr_functional _ _ _ H11 H2).
-    discriminate.
-    exfalso.
-    apply (read_instr_functional _ _ _ H11 H2).
-    discriminate.
-    exfalso.
-    apply (read_instr_functional _ _ _ H11 H2).
-    discriminate.
-    exfalso.
-    apply (read_instr_functional _ _ _ H11 H2).
-    discriminate.
-Qed.
-Theorem sequence_comp_ptrdec :
-  forall p p' q q', Compiler.compile p q -> eval p p' -> Compiler.compile p' q' ->
-              Language.read_instr p Language.PtrDec ->
-              Common.plus eval' q q'.
-Proof.
-  intros.
-  apply Common.t_base.
-  assert (Assembly.read_instr q (Assembly.Sub 1)).
-  apply (comp_newstate' p q Language.PtrDec).
-  assumption.
-  assumption.
-  assert (Assembly.read_instr q' (first_comp_instr
-                                 (Language.read_instr' p'.(Language.prog) p'.(Language.pc)))).
-  apply (comp_newstate' p' q').
-  assumption.
-  apply Language.ri.
-  reflexivity.
-  unfold eval'.
-  apply (Assembly.sub q) with (n := 1).
-  - assumption.
-  - assert (Assembly.pc q = (Compiler.new_pc p.(Language.prog) p.(Language.pc))).
-    inversion H.
-    inversion H6.
-    unfold Compiler.compile'.
-    simpl.
-    reflexivity.
-    assert (Assembly.pc q' = (Compiler.new_pc p'.(Language.prog) p'.(Language.pc))).
-    inversion H1.
-    unfold Compiler.compile' in H7.
-    inversion H1.
-    inversion H9.
-    unfold Compiler.compile'.
-    simpl.
-    reflexivity.
-    assert (Compiler.new_pc (Language.prog p') (Language.pc p') =
-            Compiler.new_pc (Language.prog p) (Language.pc p) + emitted_instr (Language.read_instr' p.(Language.prog) p.(Language.pc))).
-    inversion H2.
-    assert (emitted_instr (Language.read_instr' p.(Language.prog) p.(Language.pc)) = 1).
-    rewrite H7.
-    simpl.
-    reflexivity.
-    apply offset_newpc.
-    assumption.
-    rewrite H7 in H6.
-    inversion H2.
-    rewrite H8 in H6.
-    simpl in H6.
-    rewrite <- H5 in H6.
-    rewrite H6.
-    reflexivity.
-  - inversion H.
-    inversion H6.
-    unfold Compiler.compile'.
-    inversion H1.
-    inversion H9.
-    unfold Compiler.compile'.
-    simpl.
-    f_equal.
-    f_equal.
-    apply constant_code.
-    assumption.
-  - inversion H.
-    inversion H6.
-    unfold Compiler.compile'.
-    simpl.
-    assert (Language.mem p' = Language.mem p).
-    inversion H0.
-    exfalso.
-    apply (read_instr_functional _ _ _ H8 H2).
-    discriminate.
-    rewrite H12.
-    reflexivity.
-    exfalso.
-    apply (read_instr_functional _ _ _ H8 H2).
-    discriminate.
-    exfalso.
-    apply (read_instr_functional _ _ _ H8 H2).
-    discriminate.
-    exfalso.
-    apply (read_instr_functional _ _ _ H8 H2).
-    discriminate.
-    exfalso.
-    apply (read_instr_functional _ _ _ H8 H2).
-    discriminate.
-    exfalso.
-    apply (read_instr_functional _ _ _ H8 H2).
-    discriminate.
-    exfalso.
-    apply (read_instr_functional _ _ _ H8 H2).
-    discriminate.
-    rewrite <- H8.
-    inversion H1.
-    inversion H10.
-    unfold Compiler.compile'.
-    simpl.
-    reflexivity.
-  - assert (Assembly.b q = 0).
-    inversion H.
-    inversion H6.
-    unfold Compiler.compile'.
-    simpl.
-    reflexivity.
-    assert (Assembly.b q' = 0).
-    inversion H1.
-    inversion H7.
-    unfold Compiler.compile'.
-    simpl.
-    reflexivity.
-    rewrite H5, H6.
-    reflexivity.
-  - inversion H.
-    inversion H6.
-    unfold Compiler.compile'.
-    simpl.
-    inversion H1.
-    inversion H9.
-    unfold Compiler.compile'.
-    simpl.
-    inversion H0.
-    exfalso.
-    apply (read_instr_functional _ _ _ H11 H2).
-    discriminate.
-    rewrite H12.
-    reflexivity.
-    exfalso.
-    apply (read_instr_functional _ _ _ H11 H2).
-    discriminate.
-    exfalso.
-    apply (read_instr_functional _ _ _ H11 H2).
-    discriminate.
-    exfalso.
-    apply (read_instr_functional _ _ _ H11 H2).
-    discriminate.
-    exfalso.
-    apply (read_instr_functional _ _ _ H11 H2).
-    discriminate.
-    exfalso.
-    apply (read_instr_functional _ _ _ H11 H2).
-    discriminate.
-    exfalso.
-    apply (read_instr_functional _ _ _ H11 H2).
-    discriminate.
 Qed.
 
-Compute (Assembly.mkState [Assembly.Halt] [1] 4 4 4).
-
-Theorem sequence_comp_inc :
-  forall p p' q q', Compiler.compile p q -> eval p p' -> Compiler.compile p' q' ->
-              Language.read_instr p Language.Inc ->
-              Common.plus eval' q q'.
+Lemma comp_link_prog {n : nat} : forall p HA q, Compiler.compile_link p HA = q -> q.(Assembly.prog) = Compiler.link (@Compiler.compile'' n p.(Language.prog)).
 Proof.
   intros.
-  assert (Assembly.read_instr q (Assembly.Swap)).
-  apply (comp_newstate' p q Language.Inc); assumption.
-  assert (exists q1 q2 q3 q4 q5,
-              Assembly.read_instr q1 Assembly.Load /\
-              Assembly.read_instr q2 (Assembly.Add 1) /\
-              Assembly.read_instr q3 Assembly.Store /\
-              Assembly.read_instr q4 Assembly.Zero /\
-              Assembly.read_instr q5 Assembly.Swap /\
-              eval' q q1 /\ eval' q1 q2 /\ eval' q2 q3 /\ eval' q3 q4 /\ eval' q4 q5).
-  apply inc_instr_comp with (p := p) (p' := p'); assumption.
-  
-  destruct H4. destruct H4. destruct H4. destruct H4. destruct H4.
-  rename x into q1; rename x0 into q2; rename x1 into q3; rename x2 into q4; rename x3 into q5.
-  destruct H4.
-  destruct H5.
-  destruct H6.
-  destruct H7.
-  destruct H8.
-  destruct H9.
-  destruct H10.
-  destruct H11.
-  destruct H12.
-  apply (Common.t_trans) with (y := q1).
-  assumption.
-  apply (Common.t_trans) with (y := q2).
-  assumption.
-  apply (Common.t_trans) with (y := q3).
-  assumption.
-  apply (Common.t_trans) with (y := q4).
-  assumption.
-  apply (Common.t_trans) with (y := q5).
-  assumption.
-  apply (Common.t_base).
-  apply Assembly.swap.
-  assumption.
-  assert (Assembly.prog q4 = Assembly.prog q5).
-  inversion H13; assumption.
-  assert (Assembly.prog q3 = Assembly.prog q4).
-  inversion H12; assumption.
-  assert (Assembly.prog q2 = Assembly.prog q3).
-  inversion H11; assumption.
-  assert (Assembly.prog q1 = Assembly.prog q2).
-  inversion H10; assumption.
-  assert (Assembly.prog q = Assembly.prog q1).
-  inversion H9; assumption.
-  rewrite <- H14. rewrite <- H15. rewrite <- H16. rewrite <- H17.
-  rewrite <- H18.
-  inversion H.
-  inversion H20.
-  inversion H1.
-  inversion H23.
-  unfold Compiler.compile'.
-  simpl.
+  rewrite <- H.
+  assert (Assembly.prog
+  {|
+    Assembly.prog := Compiler.link (Assembly.prog (Compiler.compile' p HA));
+    Assembly.mem := Assembly.mem (Compiler.compile' p HA);
+    Assembly.pc := Assembly.pc (Compiler.compile' p HA);
+    Assembly.ac := Assembly.ac (Compiler.compile' p HA);
+    Assembly.b := Assembly.b (Compiler.compile' p HA)
+  |} = Compiler.link (Assembly.prog (Compiler.compile' p HA))).
+  now reflexivity.
+  unfold Compiler.compile_link.
+  rewrite H0.
   f_equal.
-  f_equal.
-  apply constant_code.
-  assumption.
-Admitted.
-Theorem sequence_comp_dec :
-  forall p p' q q', Compiler.compile p q -> eval p p' -> Compiler.compile p' q' ->
-              Language.read_instr p Language.Dec ->
-              Common.plus eval' q q'.
+Qed.
+
+
+Lemma comp_instr {n : nat} : forall (x : Fin.t n) (p : Language.program n), Compiler.compile_first p[@x] = (Compiler.compile'' p)[@Compiler.compile_index p x].
+Proof.
+Admitted. (* to be done (+ another one for linking) *)
+
+Theorem comp_correct {n : nat} :
+    forall p q, Compiler.compile p q -> 
+    forall p' (E : eval p p'), 
+    exists q', Compiler.compile p' q' /\ (Common.plus eval') q (comp_len_f (n := n) E q').
 Proof.
   intros.
-  assert (Assembly.read_instr q (Assembly.Swap)).
-  apply (comp_newstate' p q Language.Dec); assumption.
-  assert (exists q1 q2 q3 q4 q5,
-              Assembly.read_instr q1 Assembly.Load /\
-              Assembly.read_instr q2 (Assembly.Sub 1) /\
-              Assembly.read_instr q3 Assembly.Store /\
-              Assembly.read_instr q4 Assembly.Zero /\
-              Assembly.read_instr q5 Assembly.Swap /\
-              eval' q q1 /\ eval' q1 q2 /\ eval' q2 q3 /\ eval' q3 q4 /\ eval' q4 q5).
-  apply dec_instr_comp with (p := p) (p' := p'); assumption.
-  
-  destruct H4. destruct H4. destruct H4. destruct H4. destruct H4.
-  rename x into q1; rename x0 into q2; rename x1 into q3; rename x2 into q4; rename x3 into q5.
-  destruct H4.
-  destruct H5.
-  destruct H6.
-  destruct H7.
-  destruct H8.
-  destruct H9.
-  destruct H10.
-  destruct H11.
-  destruct H12.
-  apply (Common.t_trans) with (y := q1).
-  assumption.
-  apply (Common.t_trans) with (y := q2).
-  assumption.
-  apply (Common.t_trans) with (y := q3).
-  assumption.
-  apply (Common.t_trans) with (y := q4).
-  assumption.
-  apply (Common.t_trans) with (y := q5).
-  assumption.
-  apply (Common.t_base).
-  apply Assembly.swap; admit.
-Admitted.
-Theorem sequence_comp_jump :
-  forall p p' q q', Compiler.compile p q -> eval p p' -> Compiler.compile p' q' -> Language.read_instr p Language.Jump -> Common.plus eval' q q'.
-Proof.
-  intros.
-  assert (Assembly.read_instr q (Assembly.Skip)).
-  apply (comp_newstate' p q Language.Jump); assumption.
-  assert (exists n q1, Assembly.read_instr q1 (Assembly.Jump n) /\ eval' q q1).
-  apply jump_instr_comp with (p := p) (p' := p'); assumption.
-  
-  destruct H4.
-  destruct H4.
-  destruct H4.
-  rename x into n. rename x0 into q1.
+  assert (n <> 0).
+  inversion H. assumption.
+  exists (Compiler.compile_link p' H0).
+  split.
+  - apply Compiler.comp_r with (H := H0).
+    + assert (Compiler.matched (Language.prog p)).
+      inversion H.
+      assumption.
+      apply match_tr with (p := p); assumption.
+    + reflexivity.
+  - destruct E; remember (Compiler.compile_link p' H0) as q';
+    inversion H;
+    assert (Assembly.prog q = (Compiler.compile_link p H0).(Assembly.prog));
+    assert (Assembly.to_nat (Assembly.pc q) = Assembly.to_nat (Compiler.compile_index (Language.prog p) (Language.pc p)));
+    assert (Assembly.ac q = Fin.F1);
+    assert (Assembly.b q = Language.ptr p); (try (inversion H3; now reflexivity)). (*other global assertions (on q') to be added*)
+    + apply Common.t_base.
+      
+    (*todo: assert a corollary of the comp_instr lemma*)
 
-  apply (Common.t_trans) with (y := q1).
-  assumption.
-  apply (Common.t_base).
-  apply Assembly.jump with (n := n); admit.
-Admitted.
-
-(* the main theorem: *)
-
-Theorem comp_correct : Simulation.plus_forward_sim Compiler.compile eval eval'.
-Proof.
-  unfold Simulation.plus_forward_sim.
-  intros p q compileH p' evalH.
-  assert (Compiler.matched (Language.prog p')). ssimpl.
-  inversion evalH; exists (Compiler.compile' p'); (split; try (apply Compiler.comp_r); auto).
-  + apply sequence_comp_ptrinc with (p := p) (p' := p').
-    assumption. assumption. apply Compiler.comp_r. assumption. reflexivity. assumption.
-  + apply sequence_comp_ptrdec with (p := p) (p' := p').
-    assumption. assumption. apply Compiler.comp_r. assumption. reflexivity. assumption. 
-  + apply sequence_comp_inc with (p := p) (p' := p').
-    assumption. assumption. apply Compiler.comp_r. assumption. reflexivity. assumption. 
-  + apply sequence_comp_dec with (p := p) (p' := p').
-    assumption. assumption. apply Compiler.comp_r. assumption. reflexivity. assumption. 
-  + apply sequence_comp_jump with (p := p) (p' := p').
-    assumption. assumption. apply Compiler.comp_r. assumption. reflexivity. assumption.
-  + admit.
-  + admit.
-  + admit.
 Admitted.
 
 End Verification.
