src/Common.v
@@ -1,5 +1,5 @@
-Require Import List.
-Import ListNotations.
+Require Import Vector.
+Import Vector.VectorNotations.
 
 Module Common.
 
@@ -22,26 +22,5 @@ Qed.
 Inductive plus {A : Type} (R : A -> A -> Prop) : A -> A -> Prop :=
   | t_base : forall x y, R x y -> plus R x y
   | t_trans : forall x y z, R x y -> plus R y z -> plus R x z.
-
-Fixpoint take {A : Type} (n : nat) (l : list A) : list A :=
-  match n, l with
-  | 0, _ => []
-  | _, [] => []
-  | S n', h::t => h :: take n' t
-  end.
-
-Fixpoint drop {A : Type} (n : nat) (l : list A) : list A :=
-  match n, l with
-  | 0, _ => l
-  | _, [] => []
-  | S n', h::t => drop n' t
-  end.
-
-Fixpoint init {A} (l : list A) : list A :=
-  match l with
-  | [] => []
-  | cons _ [] => []
-  | cons x xs => cons x (init xs)
-  end.
 
 End Common.
