README.md
@@ -20,4 +20,5 @@
 
 ## TODO:
 
+- Use vectors instead of lists (lists make the proof too complicated to complete)
 - Complete the proof
